implement recursive_iterator with new @==>

src/lowparse/LowParse.SteelST.Recursive.fst
@@ -501,7 +501,7 @@ let jump_recursive_step_count
         SZ.v res == p.count va.contents
       )
 
-#push-options "--z3rlimit 64 --fuel 3 --ifuel 6 --query_stats"
+#push-options "--z3rlimit 128 --fuel 3 --ifuel 6 --query_stats"
 #restart-solver
 
 inline_for_extraction
@@ -789,9 +789,6 @@ let elim_recursive_as_nlist
 
 #pop-options
 
-(*
-open Steel.ST.Stick
-
 [@@__reduce__]
 let recursive_iterator0
   (p: parse_recursive_param)
@@ -801,11 +798,9 @@ let recursive_iterator0
   (n: nat)
   (va: v (parse_nlist_kind n (parse_recursive_kind p.parse_header_kind)) (nlist n p.t))
 : Tot vprop
-= (exists_ (fun (a: byte_array) -> aparse (parse_nlist n (parse_recursive p)) a va)) `stick` aparse (parse_nlist n0 (parse_recursive p)) a0 va0
+= (exists_ (fun (a: byte_array) -> aparse (parse_nlist n (parse_recursive p)) a va)) @==> aparse (parse_nlist n0 (parse_recursive p)) a0 va0
 
 let recursive_iterator
-*)
-assume val recursive_iterator
   (p: parse_recursive_param)
   (a0: byte_array)
   (n0: nat)
@@ -813,12 +808,9 @@ assume val recursive_iterator
   (n: nat)
   (va: v (parse_nlist_kind n (parse_recursive_kind p.parse_header_kind)) (nlist n p.t))
 : Tot vprop
-(*
 = recursive_iterator0 p a0 n0 va0 n va
 
 let recursive_iterator_stop
-*)
-assume val recursive_iterator_stop
   (#opened: _)
   (p: parse_recursive_param)
   (a0: byte_array)
@@ -830,16 +822,13 @@ assume val recursive_iterator_stop
 : STGhostT unit opened
    (recursive_iterator p a0 n0 va0 n va `star` aparse (parse_nlist n (parse_recursive p)) a va)
    (fun _ -> aparse (parse_nlist n0 (parse_recursive p)) a0 va0)
-(*
 = noop ();
-  stick_elim (exists_ (fun (a: byte_array) -> aparse (parse_nlist n (parse_recursive p)) a va)) (aparse (parse_nlist n0 (parse_recursive p)) a0 va0)
+  elim_implies (exists_ (fun (a: byte_array) -> aparse (parse_nlist n (parse_recursive p)) a va)) (aparse (parse_nlist n0 (parse_recursive p)) a0 va0)
 
 #push-options "--z3rlimit 32"
 
 #restart-solver
 let recursive_iterator_start
-*)
-assume val recursive_iterator_start
   (#opened: _)
   (p: parse_recursive_param)
   (a0: byte_array)
@@ -850,14 +839,13 @@ assume val recursive_iterator_start
     (fun va -> aparse (parse_nlist n0 (parse_recursive p)) a0 va `star` recursive_iterator p a0 n0 va0 n0 va)
     True
     (fun va -> va.contents == va0.contents)
-(*
 = let vb = elim_aparse _ a0 in
   Seq.slice_length (AP.contents_of' vb);
   let a = AP.gsplit a0 0sz in
   let _ = gen_elim () in
   let va = intro_aparse (parse_nlist n0 (parse_recursive p)) a in
   vpattern_rewrite (fun a -> aparse _ a _) a0;
-  stick_intro (exists_ (fun (a: byte_array) -> aparse (parse_nlist n0 (parse_recursive p)) a va)) (aparse (parse_nlist n0 (parse_recursive p)) a0 va0) (AP.arrayptr a0 _) (fun _ ->
+  intro_implies (exists_ (fun (a: byte_array) -> aparse (parse_nlist n0 (parse_recursive p)) a va)) (aparse (parse_nlist n0 (parse_recursive p)) a0 va0) (AP.arrayptr a0 _) (fun _ ->
     let a = elim_exists () in
     let vr = elim_aparse _ a in
     let vb = AP.join a0 a in
@@ -870,8 +858,6 @@ assume val recursive_iterator_start
 
 #restart-solver
 let recursive_iterator_next
-*)
-assume val recursive_iterator_next
   (#opened: _)
   (p: parse_recursive_param)
   (a0: byte_array)
@@ -905,9 +891,8 @@ assume val recursive_iterator_next
     (fun va' ->
       va'.contents == va2.contents `List.Tot.append` va3.contents
     )
-(*
 = let va' = NL.intro_nlist_sum (n2 + n3) (parse_recursive p) n2 a2 n3 a3 in
-  stick_intro (exists_ (fun (a: byte_array) -> aparse (parse_nlist (n2 + n3) (parse_recursive p)) a va')) (aparse (parse_nlist n0 (parse_recursive p)) a0 va0) (aparse p.parse_header a1 va1 `star` recursive_iterator p a0 n0 va0 n va) (fun _ ->
+  intro_implies (exists_ (fun (a: byte_array) -> aparse (parse_nlist (n2 + n3) (parse_recursive p)) a va')) (aparse (parse_nlist n0 (parse_recursive p)) a0 va0) (aparse p.parse_header a1 va1 `star` recursive_iterator p a0 n0 va0 n va) (fun _ ->
     let a2' = elim_exists () in
     let a3' = NL.elim_nlist_sum (n2 + n3) (parse_recursive p) a2' n2 n3 in
     let _ = gen_elim () in
@@ -921,7 +906,7 @@ assume val recursive_iterator_next
     rewrite
       (recursive_iterator p a0 n0 va0 n va)
       (recursive_iterator0 p a0 n0 va0 n va);
-    stick_elim (exists_ (fun (a: byte_array) -> aparse (parse_nlist n (parse_recursive p)) a va)) (aparse (parse_nlist n0 (parse_recursive p)) a0 va0)
+    elim_implies (exists_ (fun (a: byte_array) -> aparse (parse_nlist n (parse_recursive p)) a va)) (aparse (parse_nlist n0 (parse_recursive p)) a0 va0)
   );
   rewrite
     (recursive_iterator0 p a0 n0 va0 (n2 + n3) va')
@@ -929,7 +914,6 @@ assume val recursive_iterator_next
   va'
 
 #pop-options
-*)
 
 unfold
 let fold_recursive_invariant_prop0
